Compiler never fails, produces err when variable not in env

SourceToStack.v
@@ -38,77 +38,30 @@ Fixpoint lookup_depth (gamma : list (option string)) (x : string) :=
   end.
 
 Fixpoint compile_tm (gamma : list (option string)) (e : SourceLang.tm)
-    : option (list StackLang.stk_ins) :=
+    : list StackLang.stk_ins :=
   match e with
-  | SourceLang.Const v => Some [StackLang.Push (compile_val v)]
+  | SourceLang.Const v => [StackLang.Push (compile_val v)]
   | SourceLang.Var x =>
     match lookup_depth gamma x with
-    | None => None
-    | Some n => Some [StackLang.StkRef n]
+    | None => [StackLang.Err]
+    | Some n => [StackLang.StkRef n]
     end
-  | SourceLang.Prim1 op e' =>
-    match compile_tm gamma e' with
-    | None => None
-    | Some ins => Some (ins ++ [StackLang.Uop (compile_prim1 op)])
-    end
-  | SourceLang.Prim2 op e1 e2 =>
-    match compile_tm gamma e1 with
-    | None => None
-    | Some ins1 =>
-      match compile_tm (None :: gamma) e2 with
-      | None => None
-      | Some ins2 => Some (ins1 ++ ins2 ++ [compile_prim2 op])
-      end
-    end
+  | SourceLang.Prim1 op e' => compile_tm gamma e' ++ [StackLang.Uop (compile_prim1 op)]
+  | SourceLang.Prim2 op e1 e2 => compile_tm gamma e1 ++ compile_tm (None :: gamma) e2 ++ [compile_prim2 op]
   | SourceLang.App l es =>
     let fix compile_tms gamma es :=
       match es with
-      | nil => Some nil
-      | e :: es' =>
-        match compile_tm gamma e with
-        | None => None
-        | Some ins =>
-          match compile_tms (None :: gamma) es' with
-          | None => None
-          | Some inss => Some (ins ++ inss)
-          end
-        end
+      | [] => []
+      | e :: es' => compile_tm gamma e ++ compile_tms (None :: gamma) es'
       end in
-    match compile_tms gamma es with
-    | None => None
-    | Some ins => Some (ins ++ [StackLang.Call l (length es)])
-    end
-  | SourceLang.If e1 e2 e3 =>
-    match compile_tm gamma e1 with
-    | None => None
-    | Some ins1 =>
-      match compile_tm gamma e2 with
-      | None => None
-      | Some ins2 =>
-        match compile_tm gamma e3 with
-        | None => None
-        | Some ins3 => Some (ins1 ++ [StackLang.If ins2 ins3])
-        end
-      end
-    end
-  | SourceLang.Let x e1 e2 =>
-    match compile_tm gamma e1 with
-    | None => None
-    | Some ins1 =>
-      match compile_tm (Some x :: gamma) e2 with
-      | None => None
-      | Some ins2 => Some (ins1 ++ ins2)
-      end
-    end
+    compile_tms gamma es ++ [StackLang.Call l (length es)]
+  | SourceLang.If e1 e2 e3 => compile_tm gamma e1 ++ [StackLang.If (compile_tm gamma e2) (compile_tm gamma e3)]
+  | SourceLang.Let x e1 e2 => compile_tm gamma e1 ++ compile_tm (Some x :: gamma) e2
   end.
 
-Definition compile_defn (defn: SourceLang.defn) : option StackLang.stk_fun :=
+Definition compile_defn (defn: SourceLang.defn) : StackLang.stk_fun :=
   match defn with
-  | SourceLang.Defn l xs e =>
-    match compile_tm (map Some (List.rev xs)) e with
-    | None => None
-    | Some ins => Some (StackLang.Fun l (length xs) ins)
-    end
+  | SourceLang.Defn l xs e => StackLang.Fun l (length xs) (compile_tm (map Some (List.rev xs)) e)
   end.
 
 Fixpoint join_option_list {A} (lst : list (option A)) : option (list A) :=
@@ -118,24 +71,22 @@ Fixpoint join_option_list {A} (lst : list (option A)) : option (list A) :=
   | Some a :: rst => option_map (cons a) (join_option_list rst)
   end.
 
-Definition compile (src : SourceLang.prg) : option StackLang.stk_prg :=
+Definition compile (src : SourceLang.prg) : StackLang.stk_prg :=
   match src with
-  | SourceLang.Prg funs e =>
-    match join_option_list (map compile_defn funs) with
-    | None => None
-    | Some inss =>
-      match compile_tm [] e with
-      | None => None
-      | Some ins => Some (StackLang.Prg inss ins)
-      end
-    end
+  | SourceLang.Prg funs e => StackLang.Prg (map compile_defn funs) (compile_tm [] e)
   end.
 
-Theorem compiler_correctness : forall (f : nat) (prg : SourceLang.prg) (v : SourceLang.val),
-  SourceLang.eval f prg = SourceLang.Ok v ->
-  exists (stk : StackLang.stk_prg), compile prg = Some stk ->
-  exists (f' : nat), StackLang.eval f' stk = StackLang.Value (compile_val v).
+Definition compile_result (res : SourceLang.result) :=
+  match res with
+  | SourceLang.Err SourceLang.OOF => StackLang.OOF
+  | SourceLang.Err SourceLang.Error => StackLang.Error
+  | SourceLang.Ok v => StackLang.Value (compile_val v)
+  end.
+
+Theorem compiler_correctness : forall (f : nat) (prg : SourceLang.prg),
+  compile_result (SourceLang.eval f prg) = StackLang.eval f (compile prg).
 Proof.
+  intros f prg.
 Admitted.
 
 End SourceToStack.
